Finish the wn proof

wn.v
@@ -1,4 +1,4 @@
-From Hammer Require Import Tactics Hammer.
+From Hammer Require Import Tactics.
 From WR Require Import typing.
 From Coq Require Import ssreflect ssrfun ssrbool.
 From stdpp Require Import relations (rtc(..)).
@@ -16,6 +16,9 @@ with nf {n} (a : tm n) :=
   | Lam A a => nf a
   end.
 
+Lemma ne_nf n (a : tm n) : ne a -> nf a.
+Proof. elim : n / a; auto. Qed.
+
 Inductive Red {n} : tm n -> tm n -> Prop :=
 | S_β a b A :
   (* ---------------------- *)
@@ -27,7 +30,10 @@ Inductive Red {n} : tm n -> tm n -> Prop :=
   Red b0 b1 ->
   Red (App a b0) (App a b1)
 | S_Abs A a b :
+  Red a b ->
   Red (Lam A a) (Lam A b).
+
+Derive Inversion red_inv with (forall n a b, @Red n a b).
 
 #[export]Hint Constructors Red : red.
 
@@ -35,9 +41,11 @@ Definition Reds {n} := rtc (@Red n).
 
 Definition wn {n} (a : tm n) := exists b, Reds a b /\ nf b.
 
+Definition wne {n} (a : tm n) := exists b, Reds a b /\ ne b.
+
 Fixpoint Interp n (b : tm n) (A : ty) : Prop :=
   match A with
-  | I => wn b
+  | I => wne b
   | Fun A B => forall m (ξ : fin n -> fin m) (a : tm m),
       Interp m a A -> Interp m (App (ren_tm ξ b) a) B
   end.
@@ -48,6 +56,11 @@ Lemma S_β' {n} a (b t : tm n) A :
   Red (App (Lam A a) b) t.
 Proof. move=>->. apply S_β. Qed.
 
+Lemma S_Lams {n} A (a b : tm (S n)) :
+  Reds a b ->
+  Reds (Lam A a) (Lam A b).
+Proof. induction 1; hauto lq:on ctrs:Red,rtc. Qed.
+
 Lemma Red_renaming n (a b : tm n) (h : Red a b) m (ξ : fin n -> fin m) :
   Red (ren_tm ξ a) (ren_tm ξ b).
 Proof.
@@ -57,16 +70,59 @@ Proof.
   apply S_β'. by asimpl.
 Qed.
 
+Lemma Red_antirenaming n m (a : tm n) (b0 : tm m) (ξ : fin n -> fin m)
+  (h : Red (ren_tm ξ a) b0) : exists b, b0 = ren_tm ξ b /\ Red a b.
+Proof.
+  move Ea : (ren_tm ξ a) h => a0 h.
+  move : n a ξ Ea.
+  elim : m a0 b0 / h => m.
+  - move => a b A n.
+    case=>// a0 b0 ξ [].
+    case : a0 =>///= A0 a0 [] -> <- <-.
+    exists (subst_tm (b0..) a0).
+    split; first by asimpl.
+    apply S_β.
+  - move => a0 b a1 hred ih n a ξ.
+    case : a=>// t0 t1 []*; subst.
+    have : ren_tm ξ t0 = ren_tm ξ t0 by reflexivity.
+    move : ih. move/[apply].
+    case => b [? ?]; subst.
+    exists (App b t1);
+      auto with red.
+  - move => a b0 b1 h0 ih0 n []// t t0 ξ [] *. subst.
+    move : ih0 (eq_refl (ren_tm ξ t0)). move/[apply].
+    case =>b [? h]. subst.
+    exists (App t b);
+      auto with red.
+  - move => A a b h0 ih0 n []// A0 a0 ξ []*. subst.
+    move : ih0 (eq_refl (ren_tm (upRen_tm_tm ξ) a0)).
+    move /[apply].
+    case => b0 [? hb0]. subst.
+    exists (Lam A b0);
+      auto with red.
+Qed.
+
 Lemma Reds_renaming n (a b : tm n) (h : Reds a b) m (ξ : fin n -> fin m) :
   Reds (ren_tm ξ a) (ren_tm ξ b).
 Proof. elim : h; hauto lq:on ctrs:rtc use:Red_renaming. Qed.
 
+Lemma Reds_antirenaming n m (a : tm n) (b0 : tm m) (ξ : fin n -> fin m)
+  (h : Reds (ren_tm ξ a) b0) : exists b, b0 = ren_tm ξ b /\ Reds a b.
+Proof.
+  move E :  (ren_tm ξ a) h => a0 h.
+  move : a E.
+  elim : a0 b0 / h.
+  - hauto lq:on ctrs:rtc.
+  - sauto lq:on rew:off use:Red_antirenaming.
+Qed.
+
 Lemma ne_nf_renaming n (a : tm n) :
   forall m (ξ : fin n -> fin m),
-    (ne a -> ne (ren_tm ξ a)) /\ (nf a -> nf (ren_tm ξ a)).
+    (ne a <-> ne (ren_tm ξ a)) /\ (nf a <-> nf (ren_tm ξ a)).
 Proof.
   elim : n / a; solve [auto; hauto b:on].
 Qed.
+
 
 Lemma Interp_renaming n A (a : tm n) (h : Interp n a A) :
   forall m (ξ : fin n -> fin m),
@@ -135,14 +191,95 @@ Proof.
   - move => ? a i <- /=  /andP.
     case => *.
     hauto lq:on ctrs:rtc inv:tm.
-  - hauto lq:on rew:off ctrs:rtc inv:Red.
+  - move => ? a' b hred hreds ih a i ? ?. subst.
+    move E : (App a (var_tm i)) hred => c h.
+    move : E hreds ih.
+    case : c a' / h=>//.
+    + move => a0 b0 A [] -> <- hred _.
+      replace (subst_tm ((var_tm i) ..) a0) with (ren_tm (i .: idren) a0) in hred; last by substify; asimpl.
+      enough (h : exists b1, Reds a0 b1 /\ ren_tm (i .: idren) b1 = b).
+      case : h=> b1 [hb1 ?]. subst.
+      exists (Lam A b1).
+      split.
+      * auto using S_Lams.
+      * hauto l:on use:ne_nf_renaming.
+      * hauto lq:on use:Reds_antirenaming.
+    + hauto lq:on ctrs:rtc.
+    + hauto lq:on inv:Red.
 Qed.
 
-(* Need anti renaming for nf and ne *)
-
-Lemma adequacy n (a : tm n) (A : ty) (h : Interp n a A) :
-  wn a.
+Lemma S_AppLR n (a a0 b b0 : tm n) :
+  Reds a a0 ->
+  Reds b b0 ->
+  Reds (App a b) (App a0 b0).
 Proof.
-  elim : A n a h.
-  - move => /= A ihA B ihB n a ha.
-Admitted.
+  move => h. move :  b b0.
+  induction h.
+  induction 1; hauto lq:on ctrs:Red,rtc.
+  hauto lq:on ctrs:Red, rtc.
+Qed.
+
+Lemma wne_app n (a b : tm n) :
+  wne a -> wn b -> wne (App a b).
+Proof.
+  case => a0 [h00 h01].
+  case => b0 [h10 h11].
+  rewrite /wne.
+  exists (App a0 b0).
+  hauto b:on use:S_AppLR.
+Qed.
+
+Lemma adequacy (A : ty)  :
+  (forall n a, Interp n a A -> wn a) /\
+  (forall n a, wne a -> Interp n a A).
+Proof.
+  elim : A.
+  - move => /= A ihA B ihB.
+    split.
+    + move => n a ha.
+      move /(_ _ shift (var_tm var_zero) ltac:(sauto lq:on)) in ha.
+      apply ihB in ha.
+      apply ext_wn in ha.
+      rewrite /wn in ha.
+      case : ha => b [hb nfb].
+      case /Reds_antirenaming : hb => b0 [? hb0]. subst.
+      hauto l:on use:ne_nf_renaming.
+    + move => n a ha m ξ a0 ha0.
+      apply ihB.
+      have ? : wne (ren_tm ξ a)
+        by hauto q:on use:ne_nf_renaming, Reds_renaming.
+      have ? : wn a0 by sfirstorder.
+      auto using wne_app.
+  - move => /=.
+    split.
+    + sfirstorder use:ne_nf.
+    + sfirstorder.
+Qed.
+
+Lemma nf_no_step n (a : tm n) : (nf a || ne a) -> relations.nf Red a.
+Proof.
+  rewrite /relations.nf.
+  rewrite /relations.red.
+  elim : n / a.
+  - hauto lq:on inv:Red.
+  - hauto inv:Red qb:on.
+  - hauto inv:Red qb:on.
+Qed.
+
+Lemma wn_no_step n (a : tm n) : wn a -> relations.wn Red a.
+Proof.
+  hauto lqb:on use:nf_no_step unfold:relations.wn.
+Qed.
+
+Lemma stlc_wn n (Γ : context n) a A :
+  Wt Γ a A -> relations.wn Red a.
+Proof.
+  move /fundamental_lemma.
+  rewrite /SemWt.
+  move /(_ n var_tm).
+  have : γ_ok var_tm Γ.
+  rewrite /γ_ok.
+  hauto lq:on ctrs:rtc use:adequacy.
+  asimpl.
+  sfirstorder use:adequacy, wn_no_step.
+Qed.
